DynamoDbItemEncryptor/test/UpdateExpr.dfy
@@ -1,0 +1,34 @@
+include "../src/UpdateExpr.dfy"
+
+module TestUpdateExpr {
+
+  import opened DynamoDbUpdateExpr
+
+  method expect_equal<T(==)>(a: T, b: T)
+    ensures a == b
+  {
+    if a != b {
+      print "Not equal: ", a, ", ", b, "\n";
+    }
+    expect a == b;
+  }
+
+  method {:test} TestExamples() {
+    // examples from https://docs.aws.amazon.com/amazondynamodb/latest/developerguide/Expressions.UpdateExpressions.html
+    expect_equal(ExtractAttrs( "SET ProductCategory = :c, Price = :p"), ["ProductCategory", "Price"]);
+    expect_equal(ExtractAttrs( "SET RelatedItems[1] = :ri"), ["RelatedItems"]);
+    expect_equal(ExtractAttrs( "SET #pr.#5star[1] = :r5, #pr.#3star = :r3"), ["#pr", "#pr"]);
+    expect_equal(ExtractAttrs( "SET Price = Price - :p"), ["Price", "Price"]);
+    expect_equal(ExtractAttrs("SET #ri = list_append(#ri, :vals)"), ["#ri", "#ri"]);
+    expect_equal(ExtractAttrs("SET #ri = list_append(:vals, #ri)"), ["#ri", "#ri"]);
+    expect_equal(ExtractAttrs("SET Price = if_not_exists(Price, :p)"), ["Price", "Price"]);
+    expect_equal(ExtractAttrs("REMOVE Brand, InStock, QuantityOnHand"), ["Brand", "InStock", "QuantityOnHand"]);
+    expect_equal(ExtractAttrs("REMOVE RelatedItems[1], RelatedItems[2]"), ["RelatedItems", "RelatedItems"]);
+    expect_equal(ExtractAttrs("ADD QuantityOnHand :q"), ["QuantityOnHand"]);
+    expect_equal(ExtractAttrs("DELETE Color :p"), ["Color"]);
+
+    var m : ComAmazonawsDynamodbTypes.ExpressionAttributeNameMap := map["#pr" := "foo"];
+    expect_equal(ExtractAttributes("SET #pr.#5star[1] = :r5, #pr.#3star = :r3", Wrappers.Some(m)), ["foo", "foo"]);
+  }
+
+}
